more

Weidenbach_Book/IsaSAT/IsaSAT_Restart_Heuristics_LLVM.thy
@@ -2,6 +2,7 @@ theory IsaSAT_Restart_Heuristics_LLVM
   imports IsaSAT_Restart_Heuristics IsaSAT_Setup_LLVM
      IsaSAT_VMTF_State_LLVM IsaSAT_Rephase_State_LLVM
      IsaSAT_Arena_Sorting_LLVM
+     IsaSAT_Restart_Reduce_LLVM
 begin
 
 hide_fact (open) Sepref_Rules.frefI
@@ -103,49 +104,6 @@ sepref_def update_restart_phases_impl
     fold_tuple_optimizations
   by sepref
 
-sepref_def find_local_restart_target_level_fast_code
-  is \<open>uncurry find_local_restart_target_level_int\<close>
-  :: \<open>trail_pol_fast_assn\<^sup>k *\<^sub>a vmtf_remove_assn\<^sup>k \<rightarrow>\<^sub>a uint32_nat_assn\<close>
-  supply [[goals_limit=1]] length_rev[simp del]
-  unfolding find_local_restart_target_level_int_def find_local_restart_target_level_int_inv_def
-    length_uint32_nat_def vmtf_remove_assn_def trail_pol_fast_assn_def
-  apply (annot_unat_const \<open>TYPE(32)\<close>)
-   apply (rewrite at \<open>stamp (\<hole>)\<close> annot_index_of_atm)
-   apply (rewrite in \<open>(_ ! _)\<close> annot_unat_snat_upcast[where 'l=64])
-   apply (rewrite in \<open>(_ ! \<hole>)\<close> annot_unat_snat_upcast[where 'l=64])
-   apply (rewrite in \<open>(\<hole> < length _)\<close> annot_unat_snat_upcast[where 'l=64])
-  by sepref
-
-
-sepref_def find_local_restart_target_level_st_fast_code
-  is \<open>find_local_restart_target_level_st\<close>
-  :: \<open>isasat_bounded_assn\<^sup>k \<rightarrow>\<^sub>a uint32_nat_assn\<close>
-  supply [[goals_limit=1]] length_rev[simp del]
-  unfolding find_local_restart_target_level_st_alt_def isasat_bounded_assn_def PR_CONST_def
-    fold_tuple_optimizations
-  by sepref
-
-sepref_def empty_Q_fast_code
-  is \<open>empty_Q\<close>
-  :: \<open>isasat_bounded_assn\<^sup>d \<rightarrow>\<^sub>a isasat_bounded_assn\<close>
-  supply [[goals_limit=1]]
-  unfolding empty_Q_def isasat_bounded_assn_def fold_tuple_optimizations
-    heuristic_assn_def
-  by sepref
-
-
-sepref_register cdcl_twl_local_restart_wl_D_heur
-  empty_Q find_decomp_wl_st_int
-
-find_theorems count_decided_st_heur name:refine
-sepref_def cdcl_twl_local_restart_wl_D_heur_fast_code
-  is \<open>cdcl_twl_local_restart_wl_D_heur\<close>
-  :: \<open>isasat_bounded_assn\<^sup>d \<rightarrow>\<^sub>a isasat_bounded_assn\<close>
-  unfolding cdcl_twl_local_restart_wl_D_heur_def PR_CONST_def
-    fold_tuple_optimizations
-  supply [[goals_limit = 1]]
-  by sepref
-
 sepref_register upper_restart_bound_not_reached
 
 sepref_def upper_restart_bound_not_reached_fast_impl
@@ -163,60 +121,6 @@ sepref_def lower_restart_bound_not_reached_impl
   unfolding lower_restart_bound_not_reached_def PR_CONST_def isasat_bounded_assn_def
     fold_tuple_optimizations
   supply [[goals_limit = 1]]
-  by sepref
-
-definition lbd_sort_clauses_raw :: \<open>arena \<Rightarrow> vdom \<Rightarrow> nat \<Rightarrow> nat \<Rightarrow> nat list nres\<close> where
-  \<open>lbd_sort_clauses_raw arena N = pslice_sort_spec idx_cdom clause_score_less arena N\<close>
-
-definition lbd_sort_clauses :: \<open>arena \<Rightarrow> vdom \<Rightarrow> nat list nres\<close> where
-  \<open>lbd_sort_clauses arena N = lbd_sort_clauses_raw arena N 0 (length N)\<close>
-
-lemmas LBD_introsort[sepref_fr_rules] =
-  LBD_it.introsort_param_impl_correct[unfolded lbd_sort_clauses_raw_def[symmetric] PR_CONST_def]
-
-lemma quicksort_clauses_by_score_sort:
- \<open>(lbd_sort_clauses, sort_clauses_by_score) \<in>
-   Id \<rightarrow> Id \<rightarrow> \<langle>Id\<rangle>nres_rel\<close>
-   apply (intro fun_relI nres_relI)
-   subgoal for arena arena' vdom vdom'
-   by (auto simp: lbd_sort_clauses_def lbd_sort_clauses_raw_def sort_clauses_by_score_def
-       pslice_sort_spec_def le_ASSERT_iff idx_cdom_def slice_rel_def br_def
-       conc_fun_RES sort_spec_def
-       eq_commute[of _ \<open>length vdom'\<close>]
-     intro!: ASSERT_leI slice_sort_spec_refine_sort[THEN order_trans, of _ vdom vdom])
-   done
-
-
-sepref_register lbd_sort_clauses_raw
-sepref_def lbd_sort_clauses_impl
-  is \<open>uncurry lbd_sort_clauses\<close>
-  :: \<open>arena_fast_assn\<^sup>k *\<^sub>a vdom_fast_assn\<^sup>d \<rightarrow>\<^sub>a vdom_fast_assn\<close>
-  supply[[goals_limit=1]]
-  unfolding lbd_sort_clauses_def
-  apply (annot_snat_const \<open>TYPE(64)\<close>)
-  by sepref
-
-lemmas [sepref_fr_rules] =
-  lbd_sort_clauses_impl.refine[FCOMP quicksort_clauses_by_score_sort]
-
-sepref_register remove_deleted_clauses_from_avdom arena_status DELETED
-
-sepref_def remove_deleted_clauses_from_avdom_fast_code
-  is \<open>uncurry isa_remove_deleted_clauses_from_avdom\<close>
-  :: \<open>[\<lambda>(N, vdom). length vdom \<le> sint64_max]\<^sub>a arena_fast_assn\<^sup>k *\<^sub>a vdom_fast_assn\<^sup>d \<rightarrow> vdom_fast_assn\<close>
-  supply [[goals_limit=1]]
-  unfolding isa_remove_deleted_clauses_from_avdom_def
-    convert_swap gen_swap if_conn(4)
-  apply (annot_snat_const \<open>TYPE(64)\<close>)
-  by sepref
-
-
-sepref_def sort_vdom_heur_fast_code
-  is \<open>sort_vdom_heur\<close>
-  :: \<open>[\<lambda>S. length (get_clauses_wl_heur S) \<le> sint64_max]\<^sub>aisasat_bounded_assn\<^sup>d \<rightarrow> isasat_bounded_assn\<close>
-  supply sort_clauses_by_score_invI[intro]
-    [[goals_limit=1]]
-  unfolding sort_vdom_heur_def isasat_bounded_assn_def
   by sepref
 
 sepref_register max_restart_decision_lvl
@@ -255,7 +159,8 @@ sepref_register ema_get_value get_fast_ema_heur get_slow_ema_heur
 
 sepref_def restart_required_heur_fast_code
   is \<open>uncurry3 restart_required_heur\<close>
-  :: \<open>[\<lambda>(((S, _), _), _). learned_clss_count S \<le> uint64_max]\<^sub>a isasat_bounded_assn\<^sup>k *\<^sub>a uint64_nat_assn\<^sup>k*\<^sub>a uint64_nat_assn\<^sup>k *\<^sub>a uint64_nat_assn\<^sup>k \<rightarrow> word_assn\<close>
+  :: \<open>[\<lambda>(((S, _), _), _). learned_clss_count S \<le> uint64_max]\<^sub>a isasat_bounded_assn\<^sup>k *\<^sub>a
+     uint64_nat_assn\<^sup>k *\<^sub>a uint64_nat_assn\<^sup>k *\<^sub>a uint64_nat_assn\<^sup>k \<rightarrow> word_assn\<close>
   supply [[goals_limit=1]] isasat_fast_def[simp] clss_size_allcount_alt_def[simp]
     learned_clss_count_def[simp]
   unfolding restart_required_heur_def
