Weidenbach_Book/IsaSAT/IsaSAT_Restart_Reduce_LLVM.thy
@@ -1,0 +1,112 @@
+theory IsaSAT_Restart_Reduce_LLVM
+  imports IsaSAT_Restart_Reduce IsaSAT_Setup_LLVM
+begin
+
+hide_fact (open) Sepref_Rules.frefI
+no_notation Sepref_Rules.fref (\<open>[_]\<^sub>f\<^sub>d _ \<rightarrow> _\<close> [0,60,60] 60)
+no_notation Sepref_Rules.freft (\<open>_ \<rightarrow>\<^sub>f\<^sub>d _\<close> [60,60] 60)
+no_notation Sepref_Rules.freftnd (\<open>_ \<rightarrow>\<^sub>f _\<close> [60,60] 60)
+no_notation Sepref_Rules.frefnd (\<open>[_]\<^sub>f _ \<rightarrow> _\<close> [0,60,60] 60)
+
+sepref_def find_local_restart_target_level_fast_code
+  is \<open>uncurry find_local_restart_target_level_int\<close>
+  :: \<open>trail_pol_fast_assn\<^sup>k *\<^sub>a vmtf_remove_assn\<^sup>k \<rightarrow>\<^sub>a uint32_nat_assn\<close>
+  supply [[goals_limit=1]] length_rev[simp del]
+  unfolding find_local_restart_target_level_int_def find_local_restart_target_level_int_inv_def
+    length_uint32_nat_def vmtf_remove_assn_def trail_pol_fast_assn_def
+  apply (annot_unat_const \<open>TYPE(32)\<close>)
+   apply (rewrite at \<open>stamp (\<hole>)\<close> annot_index_of_atm)
+   apply (rewrite in \<open>(_ ! _)\<close> annot_unat_snat_upcast[where 'l=64])
+   apply (rewrite in \<open>(_ ! \<hole>)\<close> annot_unat_snat_upcast[where 'l=64])
+   apply (rewrite in \<open>(\<hole> < length _)\<close> annot_unat_snat_upcast[where 'l=64])
+  by sepref
+
+
+sepref_def find_local_restart_target_level_st_fast_code
+  is \<open>find_local_restart_target_level_st\<close>
+  :: \<open>isasat_bounded_assn\<^sup>k \<rightarrow>\<^sub>a uint32_nat_assn\<close>
+  supply [[goals_limit=1]] length_rev[simp del]
+  unfolding find_local_restart_target_level_st_alt_def isasat_bounded_assn_def PR_CONST_def
+    fold_tuple_optimizations
+  by sepref
+
+sepref_def empty_Q_fast_code
+  is \<open>empty_Q\<close>
+  :: \<open>isasat_bounded_assn\<^sup>d \<rightarrow>\<^sub>a isasat_bounded_assn\<close>
+  supply [[goals_limit=1]]
+  unfolding empty_Q_def isasat_bounded_assn_def fold_tuple_optimizations
+    heuristic_assn_def
+  by sepref
+
+sepref_register cdcl_twl_local_restart_wl_D_heur
+    empty_Q find_decomp_wl_st_int
+
+sepref_def cdcl_twl_local_restart_wl_D_heur_fast_code
+  is \<open>cdcl_twl_local_restart_wl_D_heur\<close>
+  :: \<open>isasat_bounded_assn\<^sup>d \<rightarrow>\<^sub>a isasat_bounded_assn\<close>
+  unfolding cdcl_twl_local_restart_wl_D_heur_def PR_CONST_def
+    fold_tuple_optimizations
+  supply [[goals_limit = 1]]
+  by sepref
+
+definition lbd_sort_clauses_raw :: \<open>arena \<Rightarrow> vdom \<Rightarrow> nat \<Rightarrow> nat \<Rightarrow> nat list nres\<close> where
+  \<open>lbd_sort_clauses_raw arena N = pslice_sort_spec idx_cdom clause_score_less arena N\<close>
+
+definition lbd_sort_clauses :: \<open>arena \<Rightarrow> vdom \<Rightarrow> nat list nres\<close> where
+  \<open>lbd_sort_clauses arena N = lbd_sort_clauses_raw arena N 0 (length N)\<close>
+
+lemmas LBD_introsort[sepref_fr_rules] =
+  LBD_it.introsort_param_impl_correct[unfolded lbd_sort_clauses_raw_def[symmetric] PR_CONST_def]
+
+lemma quicksort_clauses_by_score_sort:
+ \<open>(lbd_sort_clauses, sort_clauses_by_score) \<in>
+   Id \<rightarrow> Id \<rightarrow> \<langle>Id\<rangle>nres_rel\<close>
+   apply (intro fun_relI nres_relI)
+   subgoal for arena arena' vdom vdom'
+   by (auto simp: lbd_sort_clauses_def lbd_sort_clauses_raw_def sort_clauses_by_score_def
+       pslice_sort_spec_def le_ASSERT_iff idx_cdom_def slice_rel_def br_def
+       conc_fun_RES sort_spec_def
+       eq_commute[of _ \<open>length vdom'\<close>]
+     intro!: ASSERT_leI slice_sort_spec_refine_sort[THEN order_trans, of _ vdom vdom])
+   done
+
+
+sepref_register lbd_sort_clauses_raw
+sepref_def lbd_sort_clauses_impl
+  is \<open>uncurry lbd_sort_clauses\<close>
+  :: \<open>arena_fast_assn\<^sup>k *\<^sub>a vdom_fast_assn\<^sup>d \<rightarrow>\<^sub>a vdom_fast_assn\<close>
+  supply[[goals_limit=1]]
+  unfolding lbd_sort_clauses_def
+  apply (annot_snat_const \<open>TYPE(64)\<close>)
+  by sepref
+
+lemmas [sepref_fr_rules] =
+  lbd_sort_clauses_impl.refine[FCOMP quicksort_clauses_by_score_sort]
+
+sepref_register remove_deleted_clauses_from_avdom arena_status DELETED
+
+sepref_def remove_deleted_clauses_from_avdom_fast_code
+  is \<open>uncurry isa_remove_deleted_clauses_from_avdom\<close>
+  :: \<open>[\<lambda>(N, vdom). length vdom \<le> sint64_max]\<^sub>a arena_fast_assn\<^sup>k *\<^sub>a vdom_fast_assn\<^sup>d \<rightarrow> vdom_fast_assn\<close>
+  supply [[goals_limit=1]]
+  unfolding isa_remove_deleted_clauses_from_avdom_def
+    convert_swap gen_swap if_conn(4)
+  apply (annot_snat_const \<open>TYPE(64)\<close>)
+  by sepref
+
+
+sepref_def sort_vdom_heur_fast_code
+  is \<open>sort_vdom_heur\<close>
+  :: \<open>[\<lambda>S. length (get_clauses_wl_heur S) \<le> sint64_max]\<^sub>aisasat_bounded_assn\<^sup>d \<rightarrow> isasat_bounded_assn\<close>
+  supply sort_clauses_by_score_invI[intro]
+    [[goals_limit=1]]
+  unfolding sort_vdom_heur_def isasat_bounded_assn_def
+  by sepref
+
+
+experiment
+begin
+  export_llvm sort_vdom_heur_fast_code remove_deleted_clauses_from_avdom_fast_code
+end
+
+end
